feat: add `zbs_iop` operations  (#31)
* chore: pure semantics

* chore: theorems

RISCV/Instructions.lean
@@ -364,3 +364,35 @@ def binv (rs2_val : BitVec 64) (rs1_val : BitVec 64) : BitVec 64 :=
 -/
 def bset (rs2_val : BitVec 64) (rs1_val : BitVec 64) : BitVec 64 :=
   rs1_val ||| ((BitVec.zeroExtend 64 1#1) <<< (BitVec.extractLsb 5 0 rs2_val))
+
+/--
+  This instruction returns rs1 with a single bit cleared at the index specified in shamt.
+  The index is read from the lower log2(XLEN) bits of shamt.
+  For RV32, the encodings corresponding to shamt[5]=1 are reserved.
+-/
+def bclri (shamt : BitVec 6) (rs1_val : BitVec 64) :=
+  rs1_val &&& (~~~((BitVec.setWidth 64 1#1) <<< shamt))
+
+/--
+  This instruction returns a single bit extracted from rs1 at the index specified in shamt.
+  The index is read from the lower log2(XLEN) bits of shamt.
+  For RV32, the encodings corresponding to shamt[5]=1 are reserved.
+-/
+def bexti (shamt : BitVec 6) (rs1_val : BitVec 64) :=
+  BitVec.setWidth 64 (if (rs1_val &&& ((BitVec.setWidth 64 1#1) <<< shamt)) != 0#64 then 1#1 else 0#1)
+
+/--
+  This instruction returns rs1 with a single bit inverted at the index specified in shamt.
+  The index is read from the lower log2(XLEN) bits of shamt.
+  For RV32, the encodings corresponding to shamt[5]=1 are reserved.
+-/
+def binvi (shamt : BitVec 6) (rs1_val : BitVec 64) :=
+  rs1_val ^^^ ((BitVec.zeroExtend 64 1#1) <<< shamt)
+
+/--
+  This instruction returns rs1 with a single bit set at the index specified in shamt.
+  The index is read from the lower log2(XLEN) bits of shamt.
+  For RV32, the encodings corresponding to shamt[5]=1 are reserved.
+-/
+def bseti (shamt : BitVec 6) (rs1_val : BitVec 64) :=
+  rs1_val ||| ((BitVec.zeroExtend 64 1#1) <<< shamt)
