RISCV/SailToRV64.lean
@@ -209,6 +209,12 @@ theorem divw_eq (rs2 : regidx) (rs1 : regidx) (rd : regidx) :
     execute_DIVW rs2 rs1 rd is_unsigned
     = skeleton_binary rs2 rs1 rd (fun val1 val2 => SailRV64I.divw val2 val1 is_unsigned) := rfl
 
+/-! # "B" Extension for Bit Manipulation -/
+
 theorem zbs_rtype_eq (rs2 : regidx) (rs1 : regidx) (rd : regidx) :
     execute_ZBS_RTYPE rs2 rs1 rd op
     = skeleton_binary rs2 rs1 rd (fun val1 val2 => SailRV64I.zbs_rtype val2 val1 op) := by rfl
+
+theorem zbs_iop_eq (shamt : BitVec 6) (rs1 : regidx) (rd : regidx) :
+    execute_ZBS_IOP shamt rs1 rd op
+    = skeleton_unary rs1 rd (fun val1 => SailRV64I.zbs_iop shamt val1 op) := by rfl
